src/Init/Data/ByteArray/AdditionalOperations.lean
@@ -7,405 +7,295 @@ module
 
 prelude
 public import Init.Data.ByteArray.Basic
-public import Init.Data.Array.Lemmas
-public import Init.Data.UInt.Lemmas
-public import Init.Data.Nat.Internal
-public import Init.Grind
+import Init.Data.ByteArray.Lemmas
+import Init.Data.Array.Bootstrap
+import Init.Data.Array.Lemmas
+import Init.Omega
+import Init.ByCases
 
-set_option linter.missingDocs true
-
-public section
+@[expose] public section
 
 namespace ByteArray
 
+def SetSizeResult.setoid (origSz sz : Nat) : Setoid { x : ByteArray // x.size = sz } where
+  r a b := ∀ (i : Nat) (hi : i < sz) (hi' : i < origSz), a.1[i] = b.1[i]
+  iseqv := {
+    refl _ _ _ _ := rfl
+    symm h i hi hi' := (h i hi hi').symm
+    trans h h' i hi hi' := (h i hi hi').trans (h' i hi hi')
+  }
+
 /--
-Interprets the value in the byte array `bs` starting at index `i`
-as a 16 bit little-endian unsigned integer.
+A byte array of size `sz` where only the first `origSize` bytes are defined and the others are
+quotiented out.
 -/
-@[extern "lean_byte_array_fget_uint16_le"]
-def getUInt16LE (bs : @& ByteArray) (i : @& Nat)
-    (h : i + 2 ≤ bs.size := by get_elem_tactic) : UInt16 :=
-  let lo := bs[i]
-  let hi := bs[i + 1]
-  lo.toUInt16 ||| (hi.toUInt16 <<< 8)
+structure SetSizeResult (origSz sz : Nat) where
+  mk' :: value : Quotient (SetSizeResult.setoid origSz sz)
+
+def SetSizeResult.mk {origSz sz : Nat} (bs : ByteArray) (h : bs.size = sz) :
+    SetSizeResult origSz sz := ⟨Quotient.mk _ ⟨bs, h⟩⟩
 
 /--
-Interprets the value in the byte array `bs` starting at index `i`
-as a 16 bit big-endian unsigned integer.
--/
-@[extern "lean_byte_array_fget_uint16_be"]
-def getUInt16BE (bs : @& ByteArray) (i : @& Nat)
-    (h : i + 2 ≤ bs.size := by get_elem_tactic) : UInt16 :=
-  let hi := bs[i]
-  let lo := bs[i + 1]
-  lo.toUInt16 ||| (hi.toUInt16 <<< 8)
-
-/--
-Interprets the value in the byte array `bs` starting at index `i`
-as a 32 bit little-endian unsigned integer.
--/
-@[extern "lean_byte_array_fget_uint32_le"]
-def getUInt32LE (bs : @& ByteArray) (i : @& Nat)
-    (h : i + 4 ≤ bs.size := by get_elem_tactic) : UInt32 :=
-  let lo := bs.getUInt16LE i
-  let hi := bs.getUInt16LE (i + 2)
-  lo.toUInt32 ||| (hi.toUInt32 <<< 16)
-
-/--
-Interprets the value in the byte array `bs` starting at index `i`
-as a 32 bit big-endian unsigned integer.
--/
-@[extern "lean_byte_array_fget_uint32_be"]
-def getUInt32BE (bs : @& ByteArray) (i : @& Nat)
-    (h : i + 4 ≤ bs.size := by get_elem_tactic) : UInt32 :=
-  let hi := bs.getUInt16BE i
-  let lo := bs.getUInt16BE (i + 2)
-  lo.toUInt32 ||| (hi.toUInt32 <<< 16)
-
-/--
-Interprets the value in the byte array `bs` starting at index `i`
-as a 64 bit little-endian unsigned integer.
--/
-@[extern "lean_byte_array_fget_uint64_le"]
-def getUInt64LE (bs : @& ByteArray) (i : @& Nat)
-    (h : i + 8 ≤ bs.size := by get_elem_tactic) : UInt64 :=
-  let lo := bs.getUInt32LE i
-  let hi := bs.getUInt32LE (i + 4)
-  lo.toUInt64 ||| (hi.toUInt64 <<< 32)
-
-/--
-Interprets the value in the byte array `bs` starting at index `i`
-as a 64 bit big-endian unsigned integer.
--/
-@[extern "lean_byte_array_fget_uint64_be"]
-def getUInt64BE (bs : @& ByteArray) (i : @& Nat)
-    (h : i + 8 ≤ bs.size := by get_elem_tactic) : UInt64 :=
-  let hi := bs.getUInt32BE i
-  let lo := bs.getUInt32BE (i + 4)
-  lo.toUInt64 ||| (hi.toUInt64 <<< 32)
-
-@[simp, grind =]
-theorem size_uset {bs : ByteArray} {i : USize} {val : UInt8} (h : i.toNat < bs.size) :
-    (bs.uset i val).size = bs.size := by
-  simp [size, uset]
-
-@[simp, grind =]
-theorem size_set {bs : ByteArray} {i : Nat} {val : UInt8} (h : i < bs.size) :
-    (bs.set i val).size = bs.size := by
-  simp [size, set]
-
-/-- Writes the value into the byte array starting at index `i` in little-endian byte order. -/
-@[extern "lean_byte_array_fset_uint16_le"]
-def setUInt16LE (bs : ByteArray) (i : @& Nat) (val : UInt16)
-    (h : i + 2 ≤ bs.size := by get_elem_tactic) : ByteArray :=
-  let bs := bs.set i val.toUInt8
-  let bs := bs.set (i + 1) (val >>> 8).toUInt8 (by grind)
-  bs
-
-@[simp, grind =]
-theorem size_setUInt16LE {bs : ByteArray} {i : Nat} {val : UInt16}
-    (h : i + 2 ≤ bs.size) : (bs.setUInt16LE i val).size = bs.size := by
-  simp [setUInt16LE]
-
-/-- Writes the value into the byte array starting at index `i` in big-endian byte order. -/
-@[extern "lean_byte_array_fset_uint16_be"]
-def setUInt16BE (bs : ByteArray) (i : @& Nat) (val : UInt16)
-    (h : i + 2 ≤ bs.size := by get_elem_tactic) : ByteArray :=
-  let bs := bs.set i (val >>> 8).toUInt8
-  let bs := bs.set (i + 1) val.toUInt8 (by grind)
-  bs
-
-@[simp, grind =]
-theorem size_setUInt16BE {bs : ByteArray} {i : Nat} {val : UInt16}
-    (h : i + 2 ≤ bs.size) : (bs.setUInt16BE i val).size = bs.size := by
-  simp [setUInt16BE]
-
-/-- Writes the value into the byte array starting at index `i` in little-endian byte order. -/
-@[extern "lean_byte_array_fset_uint32_le"]
-def setUInt32LE (bs : ByteArray) (i : @& Nat) (val : UInt32)
-    (h : i + 4 ≤ bs.size := by get_elem_tactic) : ByteArray :=
-  let bs := bs.setUInt16LE i val.toUInt16
-  let bs := bs.setUInt16LE (i + 2) (val >>> 16).toUInt16 (by grind)
-  bs
-
-@[simp, grind =]
-theorem size_setUInt32LE {bs : ByteArray} {i : Nat} {val : UInt32}
-    (h : i + 4 ≤ bs.size) : (bs.setUInt32LE i val).size = bs.size := by
-  simp [setUInt32LE]
-
-/-- Writes the value into the byte array starting at index `i` in big-endian byte order. -/
-@[extern "lean_byte_array_fset_uint32_be"]
-def setUInt32BE (bs : ByteArray) (i : @& Nat) (val : UInt32)
-    (h : i + 4 ≤ bs.size := by get_elem_tactic) : ByteArray :=
-  let bs := bs.setUInt16BE i (val >>> 16).toUInt16
-  let bs := bs.setUInt16BE (i + 2) val.toUInt16 (by grind)
-  bs
-
-@[simp, grind =]
-theorem size_setUInt32BE {bs : ByteArray} {i : Nat} {val : UInt32}
-    (h : i + 4 ≤ bs.size) : (bs.setUInt32BE i val).size = bs.size := by
-  simp [setUInt32BE]
-
-/-- Writes the value into the byte array starting at index `i` in little-endian byte order. -/
-@[extern "lean_byte_array_fset_uint64_le"]
-def setUInt64LE (bs : ByteArray) (i : @& Nat) (val : UInt64)
-    (h : i + 8 ≤ bs.size := by get_elem_tactic) : ByteArray :=
-  let bs := bs.setUInt32LE i val.toUInt32
-  let bs := bs.setUInt32LE (i + 4) (val >>> 32).toUInt32 (by grind)
-  bs
-
-@[simp, grind =]
-theorem size_setUInt64LE {bs : ByteArray} {i : Nat} {val : UInt64}
-    (h : i + 8 ≤ bs.size) : (bs.setUInt64LE i val).size = bs.size := by
-  simp [setUInt64LE]
-
-/-- Writes the value into the byte array starting at index `i` in big-endian byte order. -/
-@[extern "lean_byte_array_fset_uint64_be"]
-def setUInt64BE (bs : ByteArray) (i : @& Nat) (val : UInt64)
-    (h : i + 8 ≤ bs.size := by get_elem_tactic) : ByteArray :=
-  let bs := bs.setUInt32BE i (val >>> 32).toUInt32
-  let bs := bs.setUInt32BE (i + 4) val.toUInt32 (by grind)
-  bs
-
-@[simp, grind =]
-theorem size_setUInt64BE {bs : ByteArray} {i : Nat} {val : UInt64}
-    (h : i + 8 ≤ bs.size) : (bs.setUInt64BE i val).size = bs.size := by
-  simp [setUInt64BE]
-
-theorem size_def (bs : ByteArray) : bs.size = bs.data.size := rfl
-
-@[simp]
-theorem data_extract (bs : ByteArray) (b e : Nat) :
-    (bs.extract b e).data = bs.data.extract b e := by
-  simp only [extract, copySlice, empty, emptyWithCapacity, Array.extract_zero, Array.empty_append,
-    Nat.zero_add, Array.extract_empty, Array.append_empty]
-  by_cases h : b ≤ e
-  · rw [Nat.add_sub_cancel' h]
-  · rw [Nat.sub_eq_zero_of_le (Nat.le_of_not_le h), Nat.add_zero]
-    simp only [Nat.le_refl, Array.extract_empty_of_stop_le_start, Nat.le_of_not_le h]
-
-@[simp]
-theorem size_extract (bs : ByteArray) (b e : Nat) :
-    (bs.extract b e).size = min e bs.size - b := by
-  simp [size_def]
-
-@[simp]
-theorem data_append (as bs : ByteArray) :
-    (as ++ bs).data = as.data ++ bs.data := by
-  change (as.append bs).data = _
-  simp only [ByteArray.append, copySlice, size_def, Array.extract_size, Nat.zero_add, Nat.sub_zero,
-    Nat.min_self, Nat.le_add_right, Array.extract_empty_of_size_le_start, Array.append_assoc,
-    Array.append_right_inj, Array.append_right_eq_self]
-
-@[simp]
-theorem size_append (as bs : ByteArray) : (as ++ bs).size = as.size + bs.size := by
-  simp [size_def]
-
-@[simp]
-theorem size_mk (xs : Array UInt8) : size (mk xs) = xs.size := rfl
-
-theorem getElem_def {xs : ByteArray} {i : Nat} (h : i < xs.size) : xs[i] = xs.data[i] := rfl
-
-/--
-Low-level function for growing or shrinking a byte array.
-
-Note: the contents of the bytes at the end are undefined when growing which is why
-this function returns a `Squash`.
+Low-level function for growing or shrinking a byte array. Note that the contents of the bytes
+starting at index `size` are undefined when growing.
 
 If `exact` is `false`, the capacity will be doubled when grown.
 -/
 @[extern "lean_byte_array_set_size"]
-def setSize' (bs : ByteArray) (size : @& Nat) (exact : Bool := false) :
-    Squash { b : ByteArray // b.size = size ∧ ∀ (i : Nat) h h', b[i]'h = bs[i] } := by
-  let b := bs.extract 0 size ++ mk (Array.replicate (size - bs.size) 0)
-  refine Squash.mk ⟨b, ?_⟩
-  have hsize : b.size = size := by simp [b] <;> omega
-  constructor
-  · exact hsize
-  · intro i h h'
-    rw [hsize] at h
-    rw [size_def] at h'
-    simp [b, getElem_def, h, h', Nat.lt_min]
+def setSize (bs : ByteArray) (size : @& Nat) (origSz : @& Nat) (h : bs.size = origSz)
+    (exact : Bool := false) : SetSizeResult origSz size :=
+  .mk ⟨bs.data.take size ++ Array.replicate (size - bs.size) 0⟩ (by simp [← size_data]; omega)
 
-/--
-Replaces the bytes in the range `[start, start + size)` within `bs` with `val`.
--/
-@[extern "lean_byte_array_fill"]
-def fill' (bs : ByteArray) (start size : @& Nat) (val : UInt8)
-    (h : start + size ≤ bs.size := by get_elem_tactic) : ByteArray :=
-  (mk (Array.replicate size val)).copySlice 0 bs start size
+@[elab_as_elim, induction_eliminator]
+theorem SetSizeResult.ind {origSz sz : Nat} {motive : SetSizeResult origSz sz → Prop}
+    (mk : ∀ b hb, motive (mk b hb)) (t : SetSizeResult origSz sz) : motive t := by
+  rcases t with ⟨x, hx⟩; apply mk
+
+theorem SetSizeResult.sound {origSz sz : Nat} {a ha b hb}
+    (h : ∀ i (hi : i < sz) (hi' : i < origSz), a[i] = b[i]) : @mk origSz sz a ha = mk b hb := by
+  simp only [mk, mk'.injEq]
+  exact Quotient.sound h
+
+@[inline]
+def SetSizeResult.lift {origSz sz : Nat} {α : Sort u} (f : (b : ByteArray) → b.size = sz → α)
+    (h : ∀ a ha b hb, (∀ i (hi : i < sz) (hi' : i < origSz), a[i] = b[i]) → f a ha = f b hb)
+    (x : SetSizeResult origSz sz) : α :=
+  x.value.lift (fun ⟨b, hb⟩ => f b hb) (fun ⟨a, ha⟩ ⟨b, hb⟩ => h a ha b hb)
 
 @[simp]
-theorem size_fill' {bs : ByteArray} {start size : Nat} {val : UInt8}
-    (h : start + size ≤ bs.size) : (bs.fill' start size val).size = bs.size := by
-  rw [size_def] at h
-  simp [fill', copySlice, size_def] <;> omega
+theorem SetSizeResult.lift_mk {origSz sz : Nat} {α : Sort u} {f h} {b hb} :
+    @lift origSz sz α f h (mk b hb) = f b hb := rfl
 
-theorem getElem_fill' {bs : ByteArray} {start size : Nat} {val : UInt8}
-    (h : start + size ≤ bs.size) {i : Nat} (hi : i < (bs.fill' start size val).size) :
-    (bs.fill' start size val)[i] =
-      if start ≤ i ∧ i < start + size then val else bs[i]'(size_fill' h ▸ hi) := by
-  have hstart : start ≤ bs.data.size := Nat.le_of_add_right_le h
-  have hsize : size ≤ bs.data.size := Nat.le_of_add_right_le (Nat.add_comm .. ▸ h)
-  simp only [fill', copySlice, Nat.zero_add, Array.size_replicate, Nat.sub_zero, Nat.min_self,
-    Nat.min_eq_left, Array.append_assoc, getElem_def, Array.getElem_append, Array.size_extract,
-    hstart, Array.getElem_extract, Array.getElem_replicate]
-  split
-  · simp only [Nat.not_le_of_lt ‹_›, false_and, ↓reduceIte]
-  · rename_i h'
-    replace h' := Nat.le_of_not_lt h'
-    simp only [← Nat.sub_lt_iff_lt_add', h', true_and]
+@[inline]
+def SetSizeResult.get {origSz sz : Nat} (x : SetSizeResult origSz sz) (i : Nat)
+    (hi : i < sz) (hi' : i < origSz) : UInt8 :=
+  x.lift (fun b _ => b[i]) fun _ _ _ _ hab => hab i hi hi'
+
+instance : GetElem (SetSizeResult origSz sz) Nat UInt8 (fun _ i => i < sz ∧ i < origSz) where
+  getElem x i h := x.get i h.1 h.2
+
+@[simp]
+theorem SetSizeResult.getElem_mk {i : Nat} {hi} :
+    (@mk origSz sz b hb)[i]'hi = b[i] := rfl
+
+@[simp]
+theorem SetSizeResult.getElem_setSize {b : ByteArray} {sz origSz h exact} {i : Nat} (hi) :
+    (b.setSize sz origSz h exact)[i]'hi = b[i] := by
+  rw [setSize]
+  simp only [Array.take_eq_extract, getElem_mk, getElem_eq_getElem_data]
+  rw [Array.getElem_append_left (by simp; omega)]
+  simp; rfl
+
+/-- Given the knowledge that `sz ≤ origSz`, extract the byte array out of `x`. -/
+@[inline]
+def SetSizeResult.toByteArrayOfLe (x : SetSizeResult origSz sz) (h : sz ≤ origSz) : ByteArray :=
+  x.lift (fun b _ => b) ?_
+where finally
+  intro a ha b hb hab
+  dsimp only
+  ext i hi
+  · simp [ha, hb]
+  · apply hab
+    · exact ha ▸ hi
+    · exact Nat.lt_of_lt_of_le (ha ▸ hi) h
+
+@[simp]
+theorem SetSizeResult.size_toByteArrayOfLe {x : SetSizeResult origSz sz} (h) :
+    (x.toByteArrayOfLe h).size = sz := by
+  induction x with | _ x hx; exact hx
+
+@[simp]
+theorem SetSizeResult.getElem_toByteArrayOfLe
+    {x : SetSizeResult origSz sz} {h} {i : Nat} (hi) :
+    (x.toByteArrayOfLe h)[i]'hi = x[i]'(by simp at hi; omega) := by
+  induction x; rfl
+
+/-- Returns all the defined bytes in `x`, i.e. the first `min origSz sz` bytes. -/
+def SetSizeResult.toByteArray (x : SetSizeResult origSz sz) : ByteArray :=
+  x.lift (fun b hb => (b.setSize (min origSz sz) _ hb).toByteArrayOfLe (by omega)) ?_
+where finally
+  intro a ha b hb hab
+  dsimp only
+  apply ext_getElem
+  · simp
+  · simp only [size_toByteArrayOfLe, getElem_toByteArrayOfLe, getElem_setSize]
+    intro i h _
+    exact hab i (by omega) (by omega)
+
+@[inline]
+def SetSizeResult.push (x : SetSizeResult origSz sz) (b : UInt8)
+    (h : origSz < sz := by get_elem_tactic) : SetSizeResult (origSz + 1) sz :=
+  x.lift (fun x _ => mk (x.set origSz b) (by simp [*])) ?_
+where finally
+  intro a ha b hb hab
+  apply sound
+  simp +contextual [Nat.lt_add_one_iff_lt_or_eq, or_imp, getElem_set, Nat.ne_of_gt, hab]
+
+private theorem SetSizeResult.pushBitVecLE_aux (h : origSz + nbytes ≤ sz)
+    (a : ByteArray) (ha : a.size = sz) (b : ByteArray) (hb : b.size = sz)
+    (hab : ∀ (i : Nat) (hi : i < sz), i < origSz → a[i] = b[i]) :
+    @mk (origSz + nbytes) sz (a.setBitVecLE origSz nbytes val) (by simpa using ha) =
+      mk (b.setBitVecLE origSz nbytes val) (by simpa using hb) := by
+  apply sound
+  intro i hi hi'
+  by_cases h : i < origSz
+  · simpa [getElem_setBitVecLE, Nat.not_le_of_lt h] using hab i hi h
+  · simp [getElem_setBitVecLE, hi', Nat.le_of_not_lt h]
+
+private theorem SetSizeResult.pushBitVecBE_aux (h : origSz + nbytes ≤ sz)
+    (a : ByteArray) (ha : a.size = sz) (b : ByteArray) (hb : b.size = sz)
+    (hab : ∀ (i : Nat) (hi : i < sz), i < origSz → a[i] = b[i]) :
+    @mk (origSz + nbytes) sz (a.setBitVecBE origSz nbytes val) (by simpa using ha) =
+      mk (b.setBitVecBE origSz nbytes val) (by simpa using hb) := by
+  apply sound
+  intro i hi hi'
+  by_cases h : i < origSz
+  · simpa [getElem_setBitVecBE, Nat.not_le_of_lt h] using hab i hi h
+  · simp [getElem_setBitVecBE, hi', Nat.le_of_not_lt h]
+
+@[inline]
+def SetSizeResult.pushBitVecLE (x : SetSizeResult origSz sz) (nbytes : Nat)
+    (val : BitVec (8 * nbytes)) (h : origSz + nbytes ≤ sz := by get_elem_tactic) :
+    SetSizeResult (origSz + nbytes) sz :=
+  x.lift (fun x _ => mk (x.setBitVecLE origSz nbytes val) (by simp [*])) (by apply pushBitVecLE_aux h)
+
+@[inline]
+def SetSizeResult.pushBitVecBE (x : SetSizeResult origSz sz) (nbytes : Nat)
+    (val : BitVec (8 * nbytes)) (h : origSz + nbytes ≤ sz := by get_elem_tactic) :
+    SetSizeResult (origSz + nbytes) sz :=
+  x.lift (fun x _ => mk (x.setBitVecBE origSz nbytes val) (by simp [*])) (by apply pushBitVecBE_aux h)
+
+@[inline]
+def SetSizeResult.pushUInt16LE (x : SetSizeResult origSz sz) (val : UInt16)
+    (h : origSz + 2 ≤ sz := by get_elem_tactic) : SetSizeResult (origSz + 2) sz :=
+  x.lift (fun x _ => mk (x.setUInt16LE origSz val) (by simp [*])) (by apply pushBitVecLE_aux h)
+
+@[inline]
+def SetSizeResult.pushUInt16BE (x : SetSizeResult origSz sz) (val : UInt16)
+    (h : origSz + 2 ≤ sz := by get_elem_tactic) : SetSizeResult (origSz + 2) sz :=
+  x.lift (fun x _ => mk (x.setUInt16BE origSz val) (by simp [*])) (by apply pushBitVecBE_aux h)
+
+@[inline]
+def SetSizeResult.pushUInt32LE (x : SetSizeResult origSz sz) (val : UInt32)
+    (h : origSz + 4 ≤ sz := by get_elem_tactic) : SetSizeResult (origSz + 4) sz :=
+  x.lift (fun x _ => mk (x.setUInt32LE origSz val) (by simp [*])) (by apply pushBitVecLE_aux h)
+
+@[inline]
+def SetSizeResult.pushUInt32BE (x : SetSizeResult origSz sz) (val : UInt32)
+    (h : origSz + 4 ≤ sz := by get_elem_tactic) : SetSizeResult (origSz + 4) sz :=
+  x.lift (fun x _ => mk (x.setUInt32BE origSz val) (by simp [*])) (by apply pushBitVecBE_aux h)
+
+@[inline]
+def SetSizeResult.pushUInt64LE (x : SetSizeResult origSz sz) (val : UInt64)
+    (h : origSz + 8 ≤ sz := by get_elem_tactic) : SetSizeResult (origSz + 8) sz :=
+  x.lift (fun x _ => mk (x.setUInt64LE origSz val) (by simp [*])) (by apply pushBitVecLE_aux h)
+
+@[inline]
+def SetSizeResult.pushUInt64BE (x : SetSizeResult origSz sz) (val : UInt64)
+    (h : origSz + 8 ≤ sz := by get_elem_tactic) : SetSizeResult (origSz + 8) sz :=
+  x.lift (fun x _ => mk (x.setUInt64BE origSz val) (by simp [*])) (by apply pushBitVecBE_aux h)
+
+def pushBitVecLE (x : ByteArray) (nbytes : Nat) (val : BitVec (8 * nbytes)) : ByteArray :=
+  let origSz := x.size
+  ((x.setSize (origSz + nbytes) origSz rfl).pushBitVecLE nbytes val).toByteArrayOfLe (Nat.le_refl _)
+
+def pushBitVecBE (x : ByteArray) (nbytes : Nat) (val : BitVec (8 * nbytes)) : ByteArray :=
+  let origSz := x.size
+  ((x.setSize (origSz + nbytes) origSz rfl).pushBitVecBE nbytes val).toByteArrayOfLe (Nat.le_refl _)
+
+def pushUInt16LE (x : ByteArray) (val : UInt16) : ByteArray :=
+  let origSz := x.size
+  ((x.setSize (origSz + 2) origSz rfl).pushUInt16LE val).toByteArrayOfLe (Nat.le_refl _)
+
+def pushUInt16BE (x : ByteArray) (val : UInt16) : ByteArray :=
+  let origSz := x.size
+  ((x.setSize (origSz + 2) origSz rfl).pushUInt16BE val).toByteArrayOfLe (Nat.le_refl _)
+
+def pushUInt32LE (x : ByteArray) (val : UInt32) : ByteArray :=
+  let origSz := x.size
+  ((x.setSize (origSz + 4) origSz rfl).pushUInt32LE val).toByteArrayOfLe (Nat.le_refl _)
+
+def pushUInt32BE (x : ByteArray) (val : UInt32) : ByteArray :=
+  let origSz := x.size
+  ((x.setSize (origSz + 4) origSz rfl).pushUInt32BE val).toByteArrayOfLe (Nat.le_refl _)
+
+def pushUInt64LE (x : ByteArray) (val : UInt64) : ByteArray :=
+  let origSz := x.size
+  ((x.setSize (origSz + 8) origSz rfl).pushUInt64LE val).toByteArrayOfLe (Nat.le_refl _)
+
+def pushUInt64BE (x : ByteArray) (val : UInt64) : ByteArray :=
+  let origSz := x.size
+  ((x.setSize (origSz + 8) origSz rfl).pushUInt64BE val).toByteArrayOfLe (Nat.le_refl _)
+
+@[inline]
+def SetSizeResult.fill (x : SetSizeResult origSz sz) (b : UInt8) (h : origSz ≤ sz) :
+    ByteArray :=
+  x.lift (fun x _ => x.fill origSz (sz - origSz) b) ?_
+where finally
+  intro a ha b hb hab
+  dsimp only
+  apply ext_getElem
+  · simp [ha, hb]
+  · intro i hi hi'
+    simp only [size_fill, ha] at hi
+    simp only [getElem_fill, Nat.add_sub_cancel' h, hi, and_true]
     split
     · rfl
-    · congr; omega
-
-@[ext]
-theorem ext {as bs : ByteArray} (h : as.size = bs.size)
-    (h' : ∀ (i : Nat) h h', as[i]'h = bs[i]) : as = bs := by
-  rcases as with ⟨xs⟩
-  rcases bs with ⟨ys⟩
-  congr
-  exact Array.ext h h'
-
-/--
-Grows or shrinks a byte array. When growing, additional bytes are filled with zeroes.
--/
-def setSize (bs : ByteArray) (size : Nat) (exact : Bool := false) : ByteArray :=
-  let prevSize := bs.size
-  Quot.liftOn (setSize' bs size exact)
-    (fun bs' => if h : prevSize < size then bs'.1.fill' prevSize (size - prevSize) 0 else bs'.1)
-    (fun a b _ => by
-      dsimp
-      split
-      · ext
-        · simp [a.2, b.2]
-        · simp only [getElem_fill']
-          split
-          · rfl
-          · rename_i hsize i h h' h''
-            simp only [size_fill', a.2.1] at h
-            simp only [Nat.le_of_lt hsize, Nat.add_sub_cancel', h, and_true, Nat.not_le] at h''
-            rw [a.2.2 i _ h'', b.2.2 i _ h'']
-      · ext
-        · simp [a.2, b.2]
-        · rename_i hbs i h h'
-          replace hbs := Nat.le_of_not_lt hbs
-          rw [a.2.1] at h
-          rw [a.2.2 i _ (Nat.lt_of_lt_of_le h hbs),
-            b.2.2 i _ (Nat.lt_of_lt_of_le h hbs)])
-
-@[simp, grind =]
-theorem size_setSize (bs : ByteArray) (size : Nat) (exact : Bool) :
-    (bs.setSize size exact).size = size := by
-  rw [setSize]
-  rcases bs.setSize' size exact with ⟨bs⟩
-  dsimp [Quot.liftOn]
-  split <;> simp [bs.2]
-
-theorem getElem_setSize {bs : ByteArray} {size : Nat} {exact : Bool} {i : Nat}
-    (h : i < (bs.setSize size exact).size) :
-    (bs.setSize size exact)[i] = if h : i < bs.size then bs[i] else 0 := by
-  rw [size_setSize] at h
-  simp only [setSize]
-  have ⟨q, hq⟩ : { a // bs.setSize' size exact = a } := ⟨_, rfl⟩
-  rcases q with ⟨a⟩
-  simp only [Quot.liftOn, hq]
-  split
-  · simp only [getElem_fill']
-    split
-    · rename_i h
-      rw [dif_neg (Nat.not_lt_of_le h.1)]
-    · rename_i h h' h''
-      simp only [Nat.le_of_lt h', Nat.add_sub_cancel', h, and_true, Nat.not_le] at h''
-      rw [a.2.2 i _ h'', dif_pos h'']
-  · rename_i h h'
-    replace h' := Nat.lt_of_lt_of_le h (Nat.le_of_not_lt h')
-    rw [a.2.2 i _ h', dif_pos h']
-
-theorem getElem_setSize_eq_getElem {bs : ByteArray} {size : Nat} {exact : Bool} {i : Nat}
-    {h : i < (bs.setSize size exact).size} (h' : i < bs.size) :
-    (bs.setSize size exact)[i] = bs[i] := by
-  simp only [getElem_setSize, h', ↓reduceDIte]
-
-theorem setSize'_eq_setSize (bs : ByteArray) (size : Nat) (exact : Bool) :
-    bs.setSize' size exact = Squash.mk ⟨bs.setSize size exact,
-      size_setSize .., @getElem_setSize_eq_getElem bs size exact⟩ :=
-  Subsingleton.allEq ..
-
-/--
-Creates an array that contains n repetitions of the byte v.
--/
-def replicate (n : Nat) (v : UInt8) :=
-  Quot.liftOn ((emptyWithCapacity n).setSize' n)
-    (fun x => x.1.fill' 0 n v)
-    (fun a b _ => by
-      ext
-      · simp [a.2, b.2]
-      · rename_i h
-        simp only [size_fill', b.2] at h
-        simp [getElem_fill', h])
+    · apply hab <;> omega
 
 @[simp]
-theorem _root_.Array.extract_size' {xs : Array α} {size : Nat} (h : size = xs.size) :
-    xs.extract 0 size = xs := by
-  rw [h, Array.extract_size]
+theorem SetSizeResult.size_fill {x : SetSizeResult origSz sz} {b h} :
+    (x.fill b h).size = sz := by
+  induction x with | _ x hx
+  simpa [fill] using hx
+
+theorem SetSizeResult.getElem_fill {x : SetSizeResult origSz sz} {b h} {i : Nat} {hi} :
+    (x.fill b h)[i]'hi = if h : i < origSz then x[i]'⟨by simpa using hi, h⟩ else b := by
+  induction x with | _ x hx
+  simp only [size_fill] at hi
+  simp [fill, ByteArray.getElem_fill, Nat.add_sub_cancel' h, hi, ← Nat.not_lt]; rfl
+
+def setSizeD (bs : ByteArray) (size : Nat) (exact : Bool := false) : ByteArray :=
+  let prevSz := bs.size
+  let res := bs.setSize size prevSz rfl exact
+  if h : prevSz < size then res.fill 0 (Nat.le_of_lt h) else res.toByteArrayOfLe (Nat.not_lt.mp h)
+
+@[simp, grind =]
+theorem size_setSizeD (bs : ByteArray) (size : Nat) (exact : Bool) :
+    (bs.setSizeD size exact).size = size := by
+  rw [setSizeD]
+  split <;> simp
+
+@[grind =]
+theorem getElem_setSizeD {bs : ByteArray} {size : Nat} {exact : Bool} {i : Nat}
+    (h : i < (bs.setSizeD size exact).size) :
+    (bs.setSizeD size exact)[i] = if h : i < bs.size then bs[i] else 0 := by
+  rw [size_setSizeD] at h
+  simp only [setSizeD]
+  split
+  · simp [SetSizeResult.getElem_fill]
+  · rw [dif_pos (c := i < _) (by omega)]
+    simp
+
+/-- Creates an array that contains n repetitions of the byte v. -/
+def replicate (n : Nat) (v : UInt8) :=
+  ((emptyWithCapacity n).setSize n 0 rfl).fill v (by simp)
 
 @[simp]
 theorem data_replicate (size : Nat) (value : UInt8) :
     (replicate size value).data = Array.replicate size value := by
   simp only [replicate]
-  cases (emptyWithCapacity size).setSize' size using Quot.ind with | mk a => ?_
-  simp [Quot.liftOn, fill', copySlice, ← size_def, Array.extract_empty_of_size_le_start, a.2]
+  ext
+  · simp
+  · simp [← getElem_eq_getElem_data, SetSizeResult.getElem_fill]
 
 @[simp]
 theorem size_replicate {n : Nat} {v : UInt8} : (replicate n v).size = n := by
-  simp [size_def]
+  simp [← size_data]
 
 @[simp]
 theorem getElem_replicate {i : Nat} {n : Nat} {v : UInt8} (h : i < (replicate n v).size) :
     (replicate n v)[i] = v := by
-  simp [getElem_def]
-
--- TODO: `pushUIntN{LE/BE}`
-
-/--
-Returns true if and only if the slices `[asOff, asOff + len)` in `as` and `[bsOff, bsOff + len)` in
-`bs` contain the same data.
--/
-@[extern "lean_byte_array_slice_eq"]
-def sliceEq' (as : @& ByteArray) (asOff : @& Nat) (bs : @& ByteArray) (bsOff len : @& Nat)
-    (h : asOff + len ≤ as.size := by get_elem_tactic)
-    (h' : bsOff + len ≤ bs.size := by get_elem_tactic) : Bool :=
-  as.data.extract asOff (asOff + len) == bs.data.extract bsOff (bsOff + len)
-
-/--
-Returns true if and only if the slices `[asOff, asOff + len)` in `as` and `[bsOff, bsOff + len)` in
-`bs` exist and contain the same data.
--/
-def sliceEq (as : ByteArray) (asOff : Nat) (bs : ByteArray) (bsOff : Nat) (len : Nat) : Bool :=
-  ∃ h h', sliceEq' as asOff bs bsOff len h h'
-
-/--
-Returns whether two byte arrays are equal.
-
-The notation `==` is preferred over using this function directly.
--/
-protected def beq (as bs : ByteArray) : Bool :=
-  if h : as.size = bs.size then
-    sliceEq' as 0 bs 0 as.size
-  else
-    false
-
-protected theorem beq_iff_eq {as bs : ByteArray} : as.beq bs ↔ as = bs := by
-  dsimp [ByteArray.beq]
-  split
-  · rename_i h
-    simp [sliceEq', ← size_def, h]
-    exact ⟨fun h => (h ▸ rfl : mk as.data = mk bs.data), fun h => h ▸ rfl⟩
-  · rename_i h
-    simp [ne_of_apply_ne size h]
-
-instance : DecidableEq ByteArray := fun _ _ =>
-  decidable_of_decidable_of_iff ByteArray.beq_iff_eq
+  simp [getElem_eq_getElem_data]
 
 end ByteArray
