src/Init/Data/ByteArray/Lemmas.lean
@@ -11,6 +11,8 @@ import Init.ByCases
 import Init.Data.Array.Bootstrap
 import Init.Data.Array.Extract
 import Init.Data.Array.Lemmas
+import Init.Data.BitVec.Bootstrap
+import Init.Data.BitVec.Lemmas
 import Init.Omega
 
 public section
@@ -275,10 +277,25 @@ theorem data_set {as : ByteArray} {i : Nat} {h : i < as.size} {a : UInt8} :
     (as.set i a h).data = as.data.set i a (by simpa) := by
   simp [set]
 
+@[simp]
+theorem size_set {as : ByteArray} {i : Nat} {h : i < as.size} {a : UInt8} :
+    (as.set i a h).size = as.size := by
+  simp [← size_data]
+
 theorem set_eq_push_extract_append_extract {as : ByteArray} {i : Nat} (h : i < as.size) {a : UInt8} :
     as.set i a h = (as.extract 0 i).push a ++ as.extract (i + 1) as.size := by
   ext1
   simpa using Array.set_eq_push_extract_append_extract _
+
+theorem getElem_set {as : ByteArray} {i : Nat} (h : i < as.size) {a : UInt8} {j : Nat}
+    (hj : j < (as.set i a h).size) :
+    (as.set i a h)[j] = if i = j then a else as[j]'(by simpa using hj) := by
+  simpa using Array.getElem_set h hj
+
+@[simp]
+theorem getElem_set_self {as : ByteArray} {i : Nat} (h : i < as.size) {a : UInt8} :
+    (as.set i a h)[i]'(by simpa using h) = a := by
+  simp [getElem_set]
 
 @[simp]
 theorem append_toByteArray_singleton {as : ByteArray} {a : UInt8} :
@@ -327,5 +344,308 @@ theorem extract_eq_extract_iff_getElem {as bs : ByteArray} {i j len : Nat}
     by_cases hk' : k < len
     · exact h k hk'
     · exact (by omega : k = len) ▸ h'
+
+private theorem getBitVecLE.getElem_go {bs i n h k hk acc j hj} :
+    (go bs i n h k hk acc)[j]'hj =
+      if h : j < 8 * k then acc[j] else bs[i + j / 8].toBitVec[j % 8] := by
+  fun_induction go with
+  | case1 k _ acc hk b ih =>
+    rw [ih]; split
+    · simp only [BitVec.getElem_cast, BitVec.getElem_append, b]
+      split
+      · rfl
+      · congr <;> omega
+    · rw [dif_neg (by omega)]
+  | case2 => rw [dif_pos (by omega), BitVec.getElem_cast]
+
+@[grind =]
+theorem getElem_getBitVecLE {bs : ByteArray} {i nbytes : Nat}
+    (hi : i + nbytes ≤ bs.size) (hj : j < 8 * nbytes) :
+    (getBitVecLE bs i nbytes hi)[j]'hj = bs[i + j / 8].toBitVec[j % 8] := by
+  simp [getBitVecLE, getBitVecLE.getElem_go]
+
+@[simp]
+theorem getBitVecLE_zero {bs : ByteArray} {i : Nat} (h) :
+    getBitVecLE bs i 0 h = 0#0 := BitVec.eq_nil _
+
+theorem getBitVecLE_add {bs : ByteArray} {i : Nat} (m n : Nat) (h) :
+    getBitVecLE bs i (n + m) h =
+      (getBitVecLE bs (i + m) n ++ getBitVecLE bs i m).cast (by omega) := by
+  ext i hi
+  simp +contextual only [getElem_getBitVecLE, BitVec.getElem_cast, BitVec.getElem_append,
+    Nat.sub_mul_div, left_eq_dite_iff, Nat.not_lt, Nat.sub_mul_mod]
+  intro; congr 3; omega
+
+@[simp]
+theorem getBitVecLE_one {bs : ByteArray} {i : Nat} (h) :
+    getBitVecLE bs i 1 h = bs[i].toBitVec := by
+  ext j hj
+  rw [ByteArray.getElem_getBitVecLE]
+  simp [Nat.div_eq_of_lt hj, Nat.mod_eq_of_lt hj]; rfl
+
+theorem getBitVecLE_add_one {bs : ByteArray} {i : Nat} {n : Nat} (h) :
+    getBitVecLE bs i (n + 1) h = getBitVecLE bs (i + 1) n ++ bs[i].toBitVec := by
+  rw [getBitVecLE_add]; simp; rfl
+
+theorem extractLsb'_getBitVecLE_eight {bs : ByteArray} {i : Nat} {n : Nat} {h} {k : Nat}
+    (hk : k < n) : (getBitVecLE bs i n h).extractLsb' (8 * k) 8 = bs[i + k].toBitVec := by
+  ext j hj
+  rw [BitVec.getElem_extractLsb', BitVec.getLsbD_eq_getElem (by omega), getElem_getBitVecLE]
+  simp [Nat.mul_add_div, Nat.div_eq_of_lt hj, Nat.mod_eq_of_lt hj]
+
+private theorem getBitVecBE.getMsbD_go {bs i n h k hk acc j} (hj : j < 8 * n) :
+    (go bs i n h k hk acc).getMsbD j =
+      if j < 8 * k then acc.getMsbD j else bs[i + j / 8].toBitVec.getMsbD (j % 8) := by
+  fun_induction go with
+  | case1 k _ acc hk b ih =>
+    rw [ih]; split
+    · simp only [BitVec.getMsbD_cast, BitVec.getMsbD_append, b, ← Nat.not_lt, ite_not]
+      split
+      · rfl
+      · congr <;> omega
+    · rw [if_neg (by omega)]
+  | case2 => rw [if_pos (by omega), BitVec.getMsbD_cast]
+
+theorem getMsbD_getBitVecBE {bs : ByteArray} {i nbytes : Nat}
+    (hi : i + nbytes ≤ bs.size) (hj : j < 8 * nbytes) :
+    (getBitVecBE bs i nbytes hi).getMsbD j = bs[i + j / 8].toBitVec.getMsbD (j % 8) := by
+  simp [getBitVecBE, getBitVecBE.getMsbD_go, hj]
+
+@[grind =]
+theorem getElem_getBitVecBE {bs : ByteArray} {i nbytes : Nat}
+    (hi : i + nbytes ≤ bs.size) (hj : j < 8 * nbytes) :
+    (getBitVecBE bs i nbytes hi)[j] = bs[i + nbytes - j / 8 - 1].toBitVec[j % 8] := by
+  rw [← BitVec.getLsbD_eq_getElem, BitVec.getLsbD_eq_getMsbD, getMsbD_getBitVecBE _ (by omega),
+    decide_eq_true hj, Bool.true_and, BitVec.getMsbD_eq_getLsbD, decide_eq_true (by omega),
+    Bool.true_and, BitVec.getLsbD_eq_getElem (by omega)]
+  congr <;> omega
+
+@[simp]
+theorem getBitVecBE_zero {bs : ByteArray} {i : Nat} (h) :
+    getBitVecBE bs i 0 h = 0#0 := BitVec.eq_nil _
+
+theorem getBitVecBE_add {bs : ByteArray} {i : Nat} (m n : Nat) (h) :
+    getBitVecBE bs i (n + m) h =
+      (getBitVecBE bs i m ++ getBitVecBE bs (i + m) n).cast (by omega) := by
+  apply BitVec.eq_of_getMsbD_eq
+  intro j hj
+  simp +contextual only [hj, getMsbD_getBitVecBE, BitVec.getMsbD_cast, BitVec.getMsbD_append,
+    Nat.sub_lt_iff_lt_add, ← Nat.mul_add, Nat.sub_mul_div, Nat.sub_mul_mod, ← dite_eq_ite,
+    not_false_eq_true, Nat.lt_of_not_le, right_eq_dite_iff]
+  intro; congr 3; omega
+
+@[simp]
+theorem getBitVecBE_one {bs : ByteArray} {i : Nat} (h) :
+    getBitVecBE bs i 1 h = bs[i].toBitVec := by
+  apply BitVec.eq_of_getMsbD_eq
+  intro j hj
+  rw [ByteArray.getMsbD_getBitVecBE _ hj]
+  simp [Nat.div_eq_of_lt hj, Nat.mod_eq_of_lt hj]; rfl
+
+theorem getBitVecBE_add_one {bs : ByteArray} {i : Nat} {n : Nat} (h) :
+    getBitVecBE bs i (n + 1) h =
+      (bs[i].toBitVec ++ getBitVecBE bs (i + 1) n).cast (Nat.add_comm ..) := by
+  rw [getBitVecBE_add]; simp; rfl
+
+theorem extractLsb'_getBitVecBE_eight {bs : ByteArray} {i : Nat} {n : Nat} {h} {k : Nat}
+    (hk : k < n) : (getBitVecBE bs i n h).extractLsb' (8 * k) 8 = bs[i + n - k - 1].toBitVec := by
+  ext j hj
+  rw [BitVec.getElem_extractLsb', BitVec.getLsbD_eq_getElem (by omega), getElem_getBitVecBE]
+  simp [Nat.mul_add_div, Nat.div_eq_of_lt hj, Nat.mod_eq_of_lt hj]
+
+private theorem setBitVecLE.size_go :
+    (go i nbytes val k hk acc h).size = acc.size := by
+  fun_induction go <;> simp_all +zetaDelta
+
+@[simp, grind =]
+theorem size_setBitVecLE {bs : ByteArray} {i nbytes : Nat} {val : BitVec (8 * nbytes)}
+    {hi : i + nbytes ≤ bs.size} : (bs.setBitVecLE i nbytes val hi).size = bs.size := by
+  rw [setBitVecLE, setBitVecLE.size_go]
+
+private theorem setBitVecLE.getElem_go :
+    (go i nbytes val k hk acc h)[j]'hj =
+      if i + k ≤ j ∧ j < i + nbytes then UInt8.ofBitVec (val.extractLsb' (8 * (j - i)) 8)
+      else acc[j]'(by simpa [size_go] using hj) := by
+  fun_induction go with
+  | @case1 k _ acc h hk acc' ih =>
+    unfold go
+    simp only [hk, ↓reduceDIte, ih, acc']
+    split
+    · rw [if_pos (by omega)]
+    split
+    · simp [show j = i + k by omega]
+    · rw [getElem_set, if_neg (by omega)]
+  | case2 k hk acc h hk' =>
+    unfold go
+    simp only [hk', ↓reduceDIte, right_eq_ite_iff, and_imp]
+    intros; omega
+
+@[grind =]
+theorem getElem_setBitVecLE {bs : ByteArray} {i nbytes : Nat} {val : BitVec (8 * nbytes)} {j : Nat}
+    {hi : i + nbytes ≤ bs.size} (hj : j < (bs.setBitVecLE i nbytes val hi).size) :
+    (bs.setBitVecLE i nbytes val hi)[j] =
+      if i ≤ j ∧ j < i + nbytes then UInt8.ofBitVec (val.extractLsb' (8 * (j - i)) 8)
+      else bs[j]'(by simpa using hj) := by
+  simp [setBitVecLE, setBitVecLE.getElem_go]
+
+@[simp]
+theorem setBitVecLE_zero {bs : ByteArray} {i : Nat} {val hi} :
+    bs.setBitVecLE i 0 val hi = bs := by
+  apply ByteArray.ext_getElem <;> simp +contextual [getElem_setBitVecLE, Nat.not_lt_of_le]
+
+@[simp]
+theorem setBitVecLE_one {bs : ByteArray} {i : Nat} {val hi} :
+    bs.setBitVecLE i 1 val hi = bs.set i (.ofBitVec val) hi := by
+  apply ByteArray.ext_getElem
+  · simp
+  · intro j hj hj'
+    simp only [getElem_setBitVecLE, getElem_set]
+    split
+    · simp [show i = j by omega]
+    · simp [show i ≠ j by omega]
+
+@[simp]
+theorem setBitVecLE_cast {bs : ByteArray} {i : Nat} {n n'} {val : BitVec (8 * n)} {hi}
+    (hn : 8 * n = 8 * n') : bs.setBitVecLE i n' (val.cast hn) = bs.setBitVecLE i n val := by
+  rw [Nat.mul_right_inj (by decide)] at hn
+  subst hn; rfl
+
+theorem setBitVecLE_append {bs : ByteArray} {i : Nat} {n n' k}
+    {val : BitVec (8 * n)} {val' : BitVec (8 * n')} {hk} {hi} :
+    bs.setBitVecLE i k ((val ++ val').cast hk) hi =
+      (bs.setBitVecLE i n' val').setBitVecLE (i + n') n val (by simp; omega) := by
+  apply ByteArray.ext_getElem
+  · simp
+  · intro j hj hj'
+    simp only [getElem_setBitVecLE, ← apply_ite UInt8.ofBitVec, UInt8.ofBitVec.injEq,
+      BitVec.extractLsb'_cast]
+    symm; split
+    · rw [if_pos (by omega), BitVec.extractLsb'_append_eq_of_le (by omega)]; congr; omega
+    split
+    · rw [if_pos (by omega), BitVec.extractLsb'_append_eq_of_add_le (by omega)]
+    · rw [if_neg (by omega)]
+
+theorem getBitVecLE_setBitVecLE_self {bs : ByteArray} {i nbytes : Nat} {val : BitVec (8 * nbytes)}
+    {hi} : (bs.setBitVecLE i nbytes val hi).getBitVecLE i nbytes (by simpa using hi) = val := by
+  ext j hj
+  rw [getElem_getBitVecLE, getElem_setBitVecLE, if_pos (by omega)]
+  simp [Nat.div_add_mod, hj]
+
+private theorem setBitVecBE.size_go :
+    (go i nbytes val k hk acc h).size = acc.size := by
+  fun_induction go <;> simp_all +zetaDelta
+
+@[simp, grind =]
+theorem size_setBitVecBE {bs : ByteArray} {i nbytes : Nat} {val : BitVec (8 * nbytes)}
+    {hi : i + nbytes ≤ bs.size} : (bs.setBitVecBE i nbytes val hi).size = bs.size := by
+  rw [setBitVecBE, setBitVecBE.size_go]
+
+private theorem setBitVecBE.getElem_go :
+    (go i nbytes val k hk acc h)[j]'hj =
+      if i + k ≤ j ∧ j < i + nbytes then
+        UInt8.ofBitVec (val.extractLsb' (8 * (i + nbytes - j - 1)) 8)
+      else acc[j]'(by simpa [size_go] using hj) := by
+  fun_induction go with
+  | @case1 k _ acc h hk acc' ih =>
+    unfold go
+    simp only [hk, ↓reduceDIte, ih, acc']
+    split
+    · rw [if_pos (by omega)]
+    split
+    · simp [show j = i + k by omega]; congr 2; omega
+    · rw [getElem_set, if_neg (by omega)]
+  | case2 k hk acc h hk' =>
+    unfold go
+    simp only [hk', ↓reduceDIte, right_eq_ite_iff, and_imp]
+    intros; omega
+
+@[grind =]
+theorem getElem_setBitVecBE {bs : ByteArray} {i nbytes : Nat} {val : BitVec (8 * nbytes)} {j : Nat}
+    {hi : i + nbytes ≤ bs.size} (hj : j < (bs.setBitVecBE i nbytes val hi).size) :
+    (bs.setBitVecBE i nbytes val hi)[j] =
+      if i ≤ j ∧ j < i + nbytes then
+        UInt8.ofBitVec (val.extractLsb' (8 * (i + nbytes - j - 1)) 8)
+      else bs[j]'(by simpa using hj) := by
+  simp [setBitVecBE, setBitVecBE.getElem_go]
+
+@[simp]
+theorem setBitVecBE_zero {bs : ByteArray} {i : Nat} {val hi} :
+    bs.setBitVecBE i 0 val hi = bs := by
+  apply ByteArray.ext_getElem <;> simp +contextual [getElem_setBitVecBE, Nat.not_lt_of_le]
+
+@[simp]
+theorem setBitVecBE_one {bs : ByteArray} {i : Nat} {val hi} :
+    bs.setBitVecBE i 1 val hi = bs.set i (.ofBitVec val) hi := by
+  apply ByteArray.ext_getElem
+  · simp
+  · intro j hj hj'
+    simp only [getElem_setBitVecBE, getElem_set]
+    split
+    · simp [show i = j by omega]
+    · simp [show i ≠ j by omega]
+
+@[simp]
+theorem setBitVecBE_cast {bs : ByteArray} {i : Nat} {n n'} {val : BitVec (8 * n)} {hi}
+    (hn : 8 * n = 8 * n') : bs.setBitVecBE i n' (val.cast hn) = bs.setBitVecBE i n val := by
+  rw [Nat.mul_right_inj (by decide)] at hn
+  subst hn; rfl
+
+theorem setBitVecBE_append {bs : ByteArray} {i : Nat} {n n' k}
+    {val : BitVec (8 * n)} {val' : BitVec (8 * n')} {hk} {hi} :
+    bs.setBitVecBE i k ((val ++ val').cast hk) hi =
+      (bs.setBitVecBE i n val).setBitVecBE (i + n) n' val' (by simp; omega) := by
+  apply ByteArray.ext_getElem
+  · simp
+  · intro j hj hj'
+    simp only [getElem_setBitVecBE, ← apply_ite UInt8.ofBitVec, UInt8.ofBitVec.injEq,
+      BitVec.extractLsb'_cast]
+    symm; split
+    · rw [if_pos (by omega), BitVec.extractLsb'_append_eq_of_add_le (by omega)]; congr 2; omega
+    split
+    · rw [if_pos (by omega), BitVec.extractLsb'_append_eq_of_le (by omega)]; congr; omega
+    · rw [if_neg (by omega)]
+
+theorem getBitVecBE_setBitVecBE_self {bs : ByteArray} {i nbytes : Nat} {val : BitVec (8 * nbytes)}
+    {hi} : (bs.setBitVecBE i nbytes val hi).getBitVecBE i nbytes (by simpa using hi) = val := by
+  ext j hj
+  rw [getElem_getBitVecBE, getElem_setBitVecBE, if_pos (by omega)]
+  simp only [BitVec.getElem_extractLsb']
+  rw [show 8 * _ + j % 8 = j by omega]
+  simp [hj]
+
+@[simp]
+theorem size_fill {bs : ByteArray} {start size : Nat} {val : UInt8}
+    (h : start + size ≤ bs.size) : (bs.fill start size val).size = bs.size := by
+  rw [← size_data] at h
+  simp [fill, copySlice, ← size_data] <;> omega
+
+theorem getElem_fill {bs : ByteArray} {start size : Nat} {val : UInt8}
+    (h : start + size ≤ bs.size) {i : Nat} (hi : i < (bs.fill start size val).size) :
+    (bs.fill start size val)[i] =
+      if start ≤ i ∧ i < start + size then val else bs[i]'(size_fill h ▸ hi) := by
+  have hstart : start ≤ bs.data.size := Nat.le_of_add_right_le h
+  have hsize : size ≤ bs.data.size := Nat.le_of_add_right_le (Nat.add_comm .. ▸ h)
+  simp only [fill, copySlice, Nat.zero_add, Array.size_replicate, Nat.sub_zero, Nat.min_self,
+    Nat.min_eq_left, Array.append_assoc, getElem_eq_getElem_data, Array.getElem_append, Array.size_extract,
+    hstart, Array.getElem_extract, Array.getElem_replicate]
+  split
+  · simp only [Nat.not_le_of_lt ‹_›, false_and, ↓reduceIte]; rfl
+  · rename_i h'
+    replace h' := Nat.le_of_not_lt h'
+    simp only [← Nat.sub_lt_iff_lt_add', h', true_and]
+    split
+    · rfl
+    · congr; omega
+
+protected theorem beq_iff_eq {as bs : ByteArray} : as.beq bs ↔ as = bs := by
+  dsimp [ByteArray.beq]
+  split
+  · rename_i h
+    simp [sliceEq', h, Array.extract_eq_self_of_le, ← ByteArray.ext_iff]
+  · rename_i h
+    simp [ne_of_apply_ne size h]
+
+instance : DecidableEq ByteArray := fun _ _ =>
+  decidable_of_decidable_of_iff ByteArray.beq_iff_eq
 
 end ByteArray
