src/Std/Internal/Http/Data/URI/Encoding.lean
@@ -12,6 +12,7 @@ import Init.Data.SInt.Lemmas
 import Init.Data.UInt.Lemmas
 import Init.Data.UInt.Bitwise
 import Init.Data.Array.Lemmas
+public import Init.Data.ByteArray.Lemmas
 public import Init.Data.String
 public import Std.Internal.Http.Internal.Char
 
@@ -215,8 +216,7 @@ private theorem ByteArray.toList_toByteArray (ba : ByteArray) :
   | mk data =>
     simp [List.toByteArray]
     apply ByteArray.ext
-    simp [List.toByteArray_loop_eq, ByteArray.empty]
-    decide
+    simp [List.toByteArray_loop_eq]
 
 theorem isValidUTF8_of_isAsciiByte (ba : ByteArray) (s : ba.data.all isAsciiByte) : ByteArray.IsValidUTF8 ba := by
   refine ⟨ba.data.toList.map Char.ofUInt8, ?_⟩
@@ -256,7 +256,7 @@ namespace EncodedString
 Creates an empty encoded string.
 -/
 def empty : EncodedString r :=
-  ⟨.empty, by simp []; exact fun i h => by contradiction⟩
+  ⟨.empty, by simp⟩
 
 instance : Inhabited (EncodedString r) where
   default := EncodedString.empty
@@ -409,7 +409,7 @@ namespace EncodedQueryString
 Creates an empty encoded query string.
 -/
 def empty : EncodedQueryString r :=
-  ⟨.empty, by simp; intro a h; contradiction⟩
+  ⟨.empty, by simp⟩
 
 instance : Inhabited (EncodedQueryString r) where
   default := EncodedQueryString.empty
